silveroak-opentitan/aes/Acorn/CipherEquivalence.v
@@ -34,6 +34,7 @@ Require Import Cava.Tactics.
 
 Require Import Cava.Acorn.MonadFacts.
 Require Import Cava.Acorn.CombinationalProperties.
+Require Import Cava.Acorn.SequentialProperties.
 Require Import Cava.Acorn.Acorn.
 Require Import Cava.Acorn.Identity.
 
@@ -94,7 +95,12 @@ Section WithSubroutines.
           | rewrite N2Nat.id
           | rewrite N2Bv_sized_Bv2N
           | rewrite (pairSel_mkpair_singleton (t:=Vec (Vec (Vec Bit 8) 4) 4))
-          | progress autorewrite with to_spec
+          | rewrite (pairSel_mkpair (t:=Vec (Vec (Vec Bit 8) 4) 4))
+          | rewrite fst_unpair
+          | rewrite snd_unpair
+          | rewrite mkpair_singleton
+          | progress cbn [map fst snd]
+          | progress autorewrite with to_spec vsimpl
           | progress simpl_ident ]; [ ].
   Local Ltac simplify := repeat simplify_step.
 
@@ -115,18 +121,23 @@ Section WithSubroutines.
     let i := N.to_nat (Bv2N round_i) in
     add_round_key_in_sel = nat_to_bitvec_sized 2 (if Nat.eqb i 0 then 1 else 0) ->
     round_key_sel = false ->
-    unIdent (round ([k], [rcon], [st]) [add_round_key_in_sel] [round_key_sel] [round_i])
-    = let '(k',rcon',data') := round_spec (k, rcon, st) i in
-      ([k'],[rcon'],[data']).
+    unIdent (round [(k, rcon, st)]
+                   [add_round_key_in_sel] [round_key_sel] [round_i])
+    = [round_spec (k, rcon, st) i].
   Proof.
     cbv zeta; intros. subst_lets. subst.
     cbv [key_expand_and_round cipher_round cipher_round_interleaved mcompose].
-    cbv [nat_to_bitvec_sized]. simplify.
+    simplify.
     destruct_one_match;
       compute_expr (nat_to_bitvec_sized 2 0);
       compute_expr (nat_to_bitvec_sized 2 1).
     all:rewrite (mux4_mkpair (t:=Vec (Vec (Vec Bit 8) 4) 4)).
     all:simplify.
+    all:rewrite (mkpair_singleton (A:=Vec (Vec (Vec Bit 8) 4) 4)
+                                  (B:=Vec Bit 8)).
+    all:rewrite (mkpair_singleton (A:=Pair (Vec (Vec (Vec Bit 8) 4) 4) (Vec Bit 8))
+                                  (B:=Vec (Vec (Vec Bit 8) 4) 4)).
+    all:rewrite <-surjective_pairing.
     all:reflexivity.
   Qed.
 
@@ -148,9 +159,9 @@ Section WithSubroutines.
     add_round_key_in_sel = nat_to_bitvec_sized 2 (if Nat.eqb i 0 then 1 else 0) ->
     (* round_key_sel is true if this is a "middle round" (in this context, not round 0) *)
     (round_key_sel = if Nat.eqb i 0 then false else true) ->
-    unIdent (round ([k], [rcon], [st]) [add_round_key_in_sel] [round_key_sel] [round_i])
-    = let '(k',rcon',data') := round_spec (k, rcon, st) i in
-      ([k'],[rcon'],[data']).
+    unIdent (round [(k, rcon, st)]
+                   [add_round_key_in_sel] [round_key_sel] [round_i])
+    = [round_spec (k, rcon, st) i].
   Proof.
     cbv zeta; intros. subst_lets. subst.
     cbv [key_expand_and_round
@@ -160,20 +171,24 @@ Section WithSubroutines.
     all: compute_expr (N2Bv_sized 2 (N.of_nat 0)).
     all: compute_expr (N2Bv_sized 2 (N.of_nat 1)).
     all: rewrite (mux4_mkpair (t:=Vec (Vec (Vec Bit 8) 4) 4)).
-    all: autorewrite with vsimpl.
     all: simplify.
+    all:rewrite (mkpair_singleton (A:=Vec (Vec (Vec Bit 8) 4) 4)
+                                  (B:=Vec Bit 8)).
+    all:rewrite (mkpair_singleton (A:=Pair (Vec (Vec (Vec Bit 8) 4) 4) (Vec Bit 8))
+                                  (B:=Vec (Vec (Vec Bit 8) 4) 4)).
+    all:rewrite <-surjective_pairing.
     all: reflexivity.
   Qed.
 
   Lemma key_expand_and_round_last_equiv
         is_decrypt (round_i : round_index) round_key rcon data :
-    snd (unIdent
-           (key_expand_and_round
-              (semantics:=CombinationalSemantics)
-              (round_index:=Vec Bit 4) (round_constant:=Vec Bit 8)
-              sub_bytes shift_rows mix_columns add_round_key (mix_columns [true])
-              key_expand [is_decrypt] ([round_key], [rcon], [data])
-              [[false; true]%vector] [false] [round_i]))
+    map snd (unIdent
+               (key_expand_and_round
+                  (semantics:=CombinationalSemantics)
+                  (round_index:=Vec Bit 4) (round_constant:=Vec Bit 8)
+                  sub_bytes shift_rows mix_columns add_round_key (mix_columns [true])
+                  key_expand [is_decrypt] [(round_key, rcon, data)]
+                  [[false; true]%vector] [false] [round_i]))
     = if is_decrypt
       then [add_round_key_spec (inv_shift_rows_spec (inv_sub_bytes_spec data)) round_key]
       else [add_round_key_spec (shift_rows_spec (sub_bytes_spec data)) round_key].
@@ -183,8 +198,8 @@ Section WithSubroutines.
     autorewrite with vsimpl. destruct is_decrypt; simplify; reflexivity.
   Qed.
 
-  Lemma cipher_equiv
-        (Nr : nat) (init_rcon : round_constant) (round_indices : list (list round_index))
+  Lemma cipher_loop_equiv'
+        (Nr : nat) (init_rcon : round_constant) (round_indices : list round_index)
         (num_regular_rounds round0 : round_index)
         (first_key last_key : key) (middle_keys : list key) (input : state) :
     let all_keys_and_rcons := all_keys key_expand_spec Nr (first_key, init_rcon) in
@@ -192,7 +207,133 @@ Section WithSubroutines.
     all_keys = (first_key :: middle_keys ++ [last_key])%list ->
     (* Nr must be at least two and small enough to fit in round_index size *)
     1 < Nr < 2 ^ 4 ->
-    round_indices = map (fun i => [nat_to_bitvec_sized 4 i]) (List.seq 0 (S Nr)) ->
+    round_indices = map (nat_to_bitvec_sized 4) (List.seq 0 (S Nr)) ->
+    num_regular_rounds = nat_to_bitvec_sized _ Nr ->
+    round0 = nat_to_bitvec_sized _ 0 ->
+    unIdent
+      (cipher_loop
+         (round_index:=Vec Bit 4) (round_constant:=Vec Bit 8)
+         sub_bytes shift_rows mix_columns add_round_key (mix_columns [true])
+         key_expand [num_regular_rounds] [round0] [false]
+         [first_key] [init_rcon] round_indices [input])
+    = tl (fst (fold_left_accumulate
+                 (cipher_round_interleaved
+                    add_round_key_spec' sub_bytes_spec shift_rows_spec
+                    mix_columns_spec key_expand_spec)
+                 (fun x => x)
+                 (List.seq 0 (S Nr)) (first_key, init_rcon, input))).
+    Proof.
+    cbv zeta; intro Hall_keys; intros. subst.
+    cbv [cipher_loop cipher_step mcompose]. simplify.
+
+    (* Helpful rephrasing of Nr upper bound *)
+    assert (N.of_nat Nr < 2 ^ N.of_nat 4)%N
+      by (cbn; change (2^4)%nat with 16 in *; Lia.lia).
+    pose proof (N.size_nat_le 4 (N.of_nat Nr) ltac:(Lia.lia)).
+
+    (* simplify *)
+    cbn [nor2 and2 unpeel CombinationalSemantics]. cbv [lift2].
+    cbn [bind ret Monad_ident unIdent].
+
+    (* separate the last round *)
+    erewrite loopDelayS_combinational_body_stepwise_indexed.
+    2:{ intros; repeat destruct_pair_let.
+        rewrite !(eqb_correct (t:=Vec Bit 4)).
+        rewrite !pad_combine_eq by reflexivity.
+        cbn [map combine fst snd].
+        match goal with
+        | |- context [(@unpeelVecList ?t ?n [[?x]%list;[?y]%list]%vector)] =>
+          change (@unpeelVecList t n [[x]%list;[y]%list]%vector)
+            with ([[x;y]%vector]%list)
+        end. boolsimpl.
+        match goal with
+        | |- context [(@muxPair _ _ _ ?A [?sel] ([?x], [?y]))] =>
+          rewrite (muxPair_correct (t:=A))
+        end.
+        Search key_expand_and_round.
+        simplify.
+        rewrite !(mkpair_singleton (A:=Vec (Vec (Vec Bit 8) 4) 4)
+                                   (B:=Vec Bit 8)).
+        rewrite !(mkpair_singleton (A:=Pair (Vec (Vec (Vec Bit 8) 4) 4)
+                                            (Vec Bit 8))
+                                   (B:=Vec (Vec (Vec Bit 8) 4) 4)).
+      by (intros; repeat destruct_pair_let; instantiate_app_by_reflexivity).
+    autorewrite with push_length pull_snoc natsimpl.
+    cbn [fold_left]. autorewrite with push_nth push_length natsimpl.
+
+    (* simplify round-index comparisons *)
+    rewrite !eqb_nat_to_bitvec_sized, Nat.eqb_refl by Lia.lia.
+    match goal with |- context [?n =? 0] => destr (n =? 0); [ Lia.lia | ] end.
+    boolsimpl. rewrite !pad_combine_eq by length_hammer.
+    cbn [map combine fst snd norb]. boolsimpl.
+    cbn [fold_left]. autorewrite with push_nth push_length natsimpl.
+    idtac. cbn [fold_left].
+    Set Printing Depth 10000.
+
+    (* Get all states from key expansion *)
+    map_inversion Hall_keys; subst.
+    match goal with H : @eq (list (_ * _)) _ (_ :: _ ++ [_])%list |- _ =>
+                    rename H into Hall_keys end.
+
+    (* representation change; use full key-expansion state (key * round_constant) *)
+    erewrite cipher_change_key_rep with (projkey:=@fst key round_constant)
+      by reflexivity.
+
+    erewrite <-cipher_interleaved_equiv by eassumption.
+    cbv [cipher_interleaved]. repeat destruct_pair_let.
+
+    (* prove using loop invariant *)
+    rewrite fold_left_map.
+    factor_out_loops.
+    eapply fold_left_double_invariant_seq
+      with (I:=fun _ x y => y = ([fst (fst x)], [snd (fst x)], [snd x])).
+    { (* invariant holds at start of loop *)
+      reflexivity. }
+    { (* invariant holds through loop body *)
+      intros; subst.
+      autorewrite with natsimpl in *. repeat destruct_pair_let.
+      rewrite !eqb_nat_to_bitvec_sized by Lia.lia.
+      erewrite (unpeelVecList_cons_singleton (A:=Bit))
+        by first [ Lia.lia | reflexivity
+                   | intros *; cbn [InV];
+                     autorewrite with vsimpl;
+                     intros [? | ?]; [ | tauto];
+                     subst; reflexivity ].
+      rewrite !pad_combine_eq by length_hammer.
+      cbn [combine map].
+      rewrite key_expand_and_round_equiv
+        by first [ boolsimpl; reflexivity
+                 | rewrite nat_to_bitvec_to_nat by Lia.lia;
+                   repeat destruct_one_match; (reflexivity || Lia.lia) ].
+      rewrite nat_to_bitvec_to_nat by Lia.lia.
+      cbv [cipher_round_interleaved].
+      repeat destruct_pair_let. subst_lets. cbn [fst snd].
+      rewrite <-surjective_pairing.
+      reflexivity. }
+    { (* invariant implies postcondition *)
+      intros; subst. cbn [fst snd].
+      erewrite (unpeelVecList_cons_singleton (A:=Bit))
+        by first [ Lia.lia | reflexivity
+                   | intros *; cbn [InV];
+                     autorewrite with vsimpl;
+                     intros [? | ?]; [ | tauto];
+                     subst; reflexivity ].
+      rewrite !pad_combine_eq by length_hammer.
+      cbn [combine map fst snd].
+      rewrite key_expand_and_round_last_equiv.
+      reflexivity. }
+  Qed.
+
+  Lemma cipher_equiv
+        (Nr : nat) (init_rcon : round_constant) (round_indices : list round_index)
+        (num_regular_rounds round0 : round_index)
+        (first_key last_key : key) (middle_keys : list key) (input : state) :
+    let all_keys_and_rcons := all_keys key_expand_spec Nr (first_key, init_rcon) in
+    let all_keys := List.map fst all_keys_and_rcons in
+    all_keys = (first_key :: middle_keys ++ [last_key])%list ->
+    (* Nr must be at least two and small enough to fit in round_index size *)
+    1 < Nr < 2 ^ 4 ->
+    round_indices = map (nat_to_bitvec_sized 4) (List.seq 0 (S Nr)) ->
     num_regular_rounds = nat_to_bitvec_sized _ Nr ->
     round0 = nat_to_bitvec_sized _ 0 ->
     unIdent
@@ -218,13 +359,19 @@ Section WithSubroutines.
     cbn [bind ret Monad_ident unIdent].
 
     (* separate the last round *)
-    rewrite foldLM_ident_fold_left.
-    autorewrite with pull_snoc natsimpl.
+    erewrite loopDelayS_stepwise_indexed
+      by (intros; repeat destruct_pair_let; instantiate_app_by_reflexivity).
+    autorewrite with push_length pull_snoc natsimpl.
+    cbn [fold_left]. autorewrite with push_nth push_length natsimpl.
 
     (* simplify round-index comparisons *)
     rewrite !eqb_nat_to_bitvec_sized, Nat.eqb_refl by Lia.lia.
     match goal with |- context [?n =? 0] => destr (n =? 0); [ Lia.lia | ] end.
-    boolsimpl.
+    boolsimpl. rewrite !pad_combine_eq by length_hammer.
+    cbn [map combine fst snd norb]. boolsimpl.
+    cbn [fold_left]. autorewrite with push_nth push_length natsimpl.
+    idtac. cbn [fold_left].
+    Set Printing Depth 10000.
 
     (* Get all states from key expansion *)
     map_inversion Hall_keys; subst.
